Added more documentation comments

src/Untyped/Beta.v
@@ -1,5 +1,8 @@
-(* Add LoadPath "~/src/tractatus/src/Untyped/". *)
+Add LoadPath "./src/Untyped/".
 
+Module src.
+Module Untyped.
+Module Beta.
 Require Import String.
 Require Import Coq.Arith.EqNat.
 Require Import Coq.Relations.Relation_Operators.
@@ -7,7 +10,6 @@ Require Import Coq.Relations.Relation_Operators.
 Require Import Syntax.
 Require Import Substitute.
 
-Module Export Beta.
 (**
   Beta reduction amounts to taking a term of the form
   [(lambda x . b) t] and producing [[x:=t]b]. If the term given
@@ -45,6 +47,11 @@ Fixpoint BetaNF (M:Term) : Prop :=
   | App M' N => (BetaNF M')/\(BetaNF N)
   end.
 
+(** What expression wouldn't be in Beta normal form? One that would never
+    terminate. For example, the [Combinator.Omega] evaluates to itself after
+    beta reduction, so if we tried repeatedly beta reducing...we'll end up in
+    an infinite loop. Which may be bad.
+*)
 Example Omega_combinator_isnt_beta_nf :
   ~(BetaNF Combinator.Omega).
 Proof.
@@ -57,25 +64,57 @@ Proof.
   simpl; tauto. (* And it's obvious. *)
 Qed.
 
+(** * Values
+
+We would like to think of Beta reduction as one step in an abstract
+"processor". A value would be where the Beta reduction would stop after
+finitely many steps. So we'll just take [BetaNF] as the criteria for
+determining if a [Term] is a value or not.
+*)
 Definition value (t:Term) : Prop := BetaNF t.
 Hint Unfold value.
-Reserved Notation "t1 '⇒' t2" (at level 40).
+
+(** * Small-Step Operational Semantics
+
+We can explicitly state the rules for our "abstract processor".
+
+*)
+
+(** 
+[[
+                               value v
+                      --------------------------                    (ST_AppAbs)
+                        (λx.t) v ==> [x:=v]t
+
+                              t1 ==> t1'
+                           ----------------                           (ST_App1)
+                           t1 t2 ==> t1' t2
+
+                              value v
+                              t2 ==> t2'
+                            --------------                           (ST_App2)
+                            v t2 ==> v t2'
+]]
+*)
+Reserved Notation "t1 '==>' t2" (at level 40).
 
 Inductive step : Term -> Term -> Prop :=
   | ST_AppAbs : forall t v,
          value v ->
-         (App (Lam t) v) ⇒ [BId 0:=v]t
+         (App (Lam t) v) ==> [BId 0:=v]t (* Beta reduction, more or less *)
   | ST_App1 : forall t1 t1' t2,
-         t1 ⇒ t1' ->
-         App t1 t2 ⇒ App t1' t2
+         t1 ==> t1' ->
+         App t1 t2 ==> App t1' t2
   | ST_App2 : forall v1 t2 t2',
          value v1 ->
-         t2 ⇒ t2' ->
-         App v1 t2 ⇒ App v1 t2'
-where "t1 '⇒' t2" := (step t1 t2).
+         t2 ==> t2' ->
+         App v1 t2 ==> App v1 t2'
+where "t1 '==>' t2" := (step t1 t2).
 Hint Constructors step.
 
 Notation multistep := (clos_refl_trans step).
-Notation "t1 '⇒*' t2" := (multistep t1 t2) (at level 40).
+Notation "t1 '==>*' t2" := (multistep t1 t2) (at level 40).
 
 End Beta.
+End Untyped.
+End src.
